Strata/DDM/Integration/Lean.lean
@@ -4,8 +4,6 @@
   SPDX-License-Identifier: Apache-2.0 OR MIT
 -/
 
-import Strata.DDM.Elab
-import Strata.DDM.Integration.Lean.Env
 import Strata.DDM.Integration.Lean.Gen
 import Strata.DDM.Integration.Lean.Quote
 import Strata.DDM.Integration.Lean.ToExpr
@@ -77,7 +75,7 @@ def strataDialectImpl: Lean.Elab.Command.CommandElab := fun (stx : Syntax) => do
   let loaded := (dialectExt.getState (←Lean.getEnv)).loaded
   let (_, d, s) ← Strata.Elab.elabDialect {} loaded inputCtx p e
   if !s.errors.isEmpty then
-    for (stx, e) in s.errors do
+    for e in s.errors do
       logMessage e
     return
   -- Add dialect to command environment
@@ -98,7 +96,7 @@ def strataProgramImpl : TermElab := fun stx tp => do
   | .ok pgm =>
     return toExpr pgm
   | .error errors =>
-    for (stx, e) in errors do
+    for e in errors do
       logMessage e
     return mkApp2 (mkConst ``sorryAx [1]) (toTypeExpr Program) (toExpr true)
 
